Introduce rely/guar reasoning and identify completeness issue for SC

PSC.thy
@@ -4,59 +4,189 @@ begin
 
 type_synonym ('a,'b) m = "'a \<Rightarrow> 'b"
 
+section \<open>List Utilities\<close>
+
+lemma post_preE:
+  assumes "A @ [e] = s # B"
+  obtains (empty) "A = []" "B = []" "e = s" |
+          (mid) l where "A = s # l" "B = l @ [e]"
+  using assms by (cases A) auto
+
+lemma pre_postE:
+  assumes "s # B = A @ [e]"
+  obtains (empty) "A = []" "B = []" "e = s" |
+          (mid) l where "A = s # l" "B = l @ [e]"
+  using assms by (cases A) auto
+
+subsection \<open>lastf\<close>
+
+fun lastf
+  where 
+    "lastf f [] = None" |
+    "lastf f (e#l) = (case lastf f l of Some v \<Rightarrow> Some v | None \<Rightarrow> (if f e then Some e else None))"
+
+lemma lastf_none [simp]:
+  assumes "\<forall>x \<in> set l. \<not> f x"
+  shows "lastf f l = None"
+  using assms by (induct l) (auto)
+
+lemma lastf_append [simp]:
+  assumes "f a"
+  shows "lastf f (p @ [a]) = Some a"
+  using assms by (induct p) (auto)
+
+lemma lastf_concat [simp]:
+  "lastf f (p@l) = (case lastf f l of Some v \<Rightarrow> Some v  | None \<Rightarrow> lastf f p)"
+  by (induct p) (auto split: option.splits)
+
+lemma lastf_some [intro]:
+  "lastf f l = Some a \<Longrightarrow> f a"
+  by (induct l) (auto split: option.splits if_splits)
+
+section \<open>Events\<close>
+
 datatype ('a,'b) event =
   W "'a" "'b" |
   R "'a" "'b" |
   MF |
   FL "'a" |
-  FO "'a"
+  FO "'a" |
+  RMW "'a" "'b" "'b" |
+  RMF "'a" "'b"
+
+section \<open>Persistent Buffer Events\<close>
 
 datatype ('t,'b) pevent =
   PFO "'t" |
   PW "'b"
 
-type_synonym ('t,'b) pbuffer = "('t,'b) pevent list"
+fun isPW :: "('t,'b) pevent \<Rightarrow> bool"
+  where 
+    "isPW (PW _) = True" |
+    "isPW _ = False"
 
-type_synonym ('a,'t,'b) pbuffers = "'a \<Rightarrow> ('t,'b) pevent list"
+fun isPFO :: "('t,'b) pevent \<Rightarrow> bool"
+  where 
+    "isPFO (PFO _) = True" | 
+    "isPFO _ = False"
 
-fun last_write :: "('t,'b) pbuffer \<Rightarrow> 'b option"
-  where
-    "last_write [] = None" |
-    "last_write (PW b#xs) = (case last_write xs of Some v \<Rightarrow> Some v | None \<Rightarrow> Some b)" |
-    "last_write (a#xs) = last_write xs"
+section \<open>State\<close>
 
-fun get :: "('a,'b) m \<Rightarrow> ('t,'b) pbuffer \<Rightarrow> 'a \<Rightarrow> 'b"
-  where
-    "get m p a = (case last_write p of Some v \<Rightarrow> v | None \<Rightarrow> m a)"
+record ('a,'t,'b) state =
+  persistent :: "('a,'b) m"
+  buffers :: "'a \<Rightarrow> ('t,'b) pevent list"
 
-definition bufapp :: "('a,'t,'b) pbuffers \<Rightarrow> 'a \<Rightarrow> ('t,'b) pevent \<Rightarrow> ('a,'t,'b) pbuffers"
-  where "bufapp P x e \<equiv> P(x := (P x)@[e])"
+definition get :: "('a,'t,'b) state \<Rightarrow> 'a \<Rightarrow> 'b"
+  where "get m a \<equiv> (case lastf isPW (buffers m a) of Some (PW v) \<Rightarrow> v | _ \<Rightarrow> persistent m a)"
 
-type_synonym ('a,'t,'b) state = "('a,'b) m \<times> ('a,'t,'b) pbuffers"
+abbreviation persistent_set :: "('a,'t,'b) state \<Rightarrow> 'a \<Rightarrow> 'b \<Rightarrow> ('a,'t,'b) state" 
+  ("_\<lbrakk>_ \<^sub>p= _\<rbrakk>" [900,0,0] 900)
+  where "persistent_set m x v \<equiv> persistent_update (\<lambda>b. b(x := v)) m"
 
-abbreviation persistent :: "('a,'t,'b) state \<Rightarrow> ('a,'b) m"
-  where "persistent m \<equiv> fst m"
+abbreviation buffer_set :: "('a,'t,'b) state \<Rightarrow> 'a \<Rightarrow> ('t,'b) pevent list \<Rightarrow> ('a,'t,'b) state" 
+  ("_\<lbrakk>_ \<^sub>b= _\<rbrakk>" [900,0,0] 900)
+  where "buffer_set m x p \<equiv> buffers_update (\<lambda>b. b(x := p)) m"
 
-abbreviation buffers :: "('a,'t,'b) state \<Rightarrow> ('a,'t,'b) pbuffers"
-  where "buffers m \<equiv> snd m"
+abbreviation buffer_app :: "('a,'t,'b) state \<Rightarrow> 'a \<Rightarrow> ('t,'b) pevent \<Rightarrow> ('a,'t,'b) state" 
+  ("_\<lbrakk>_ \<^sub>@= _\<rbrakk>" [900,0,0] 900)
+  where "buffer_app m x e \<equiv> m\<lbrakk>x \<^sub>b= (buffers m x)@[e] \<rbrakk>"
 
-definition view :: "('a,'b) m \<times> ('a,'t,'b) pbuffers \<Rightarrow> ('a,'b) m"
-  where "view m a \<equiv> get (persistent m) (buffers m a) a"
+lemma get_no_pw[simp]:
+  assumes "\<forall>e \<in> set (buffers m x). \<not> isPW e"
+  shows "get m x = persistent m x"
+  using assms by (auto simp: get_def fun_eq_iff split: option.splits pevent.splits)
+
+lemma get_no_pw'[simp]:
+  assumes "\<forall>e \<in> set (buffers m x). \<not> isPW e"
+  shows "get (m\<lbrakk>x \<^sub>p= v\<rbrakk>) = (get m)(x := v)"
+  using assms by (auto simp: get_def fun_eq_iff split: option.splits pevent.splits)
+
+lemma [simp]:
+  shows "(lastf isPW p = Some (PFO v)) = False"
+  by (rule iffI,drule lastf_some) auto
+
+lemma get_simps [simp]:
+  "x \<noteq> y \<Longrightarrow> get (m\<lbrakk>y \<^sub>b= p\<rbrakk>) x = get m x"
+  "x \<noteq> y \<Longrightarrow> get (m\<lbrakk>y \<^sub>p= a\<rbrakk>) x = get m x"
+
+  "get (m\<lbrakk>x \<^sub>@= PW v\<rbrakk>) = (get m)(x := v)"
+  "get (m\<lbrakk>x \<^sub>@= PFO t\<rbrakk>) = get m"
+
+  "(get (m\<lbrakk>x \<^sub>p= v\<rbrakk>))(x := v) = (get m)(x := v)"
+  "get (m\<lbrakk>x \<^sub>b= []\<rbrakk>) = (get m)(x := persistent m x)"
+  by (auto simp: get_def fun_eq_iff split: option.splits pevent.splits)
+
+lemma [simp]:
+  "(\<lambda>b. b(y := c)) \<circ> (\<lambda>b. b(x := g b)) = (\<lambda>b. b(x := g b, y := c))"
+  by auto
+
+lemma redundant_buffer_set [simp]:
+  assumes "buffers m y = p"
+  shows "m\<lbrakk>y \<^sub>b= p\<rbrakk> = m"
+  using assms by auto
+
+lemma pers_buf_twist:
+  "buffers_update g (persistent_update f m) = persistent_update f (buffers_update g m)"
+  by (metis surjective update_convs(1,2))
+
+subsection \<open>remainder\<close>
+
+fun rem :: "'t \<Rightarrow> ('t,'b) pevent list \<Rightarrow> ('t,'b) pevent list"
+  where 
+    "rem t [] = []" |
+    "rem t (a#xs) = (if PFO t \<in> set xs then rem t xs else if a = PFO t then xs else a#xs)"
+
+lemma [simp]:
+  "PFO s \<notin> set (rem s l)"
+  by (induct l) auto
+
+section \<open>Semantics\<close>
 
 inductive step :: "('a,'t,'b) state \<Rightarrow> 't \<Rightarrow> ('a,'b) event \<Rightarrow> ('a,'t,'b) state \<Rightarrow> bool"
   ("\<langle>_\<rangle> -_,_\<rightarrow> \<langle>_\<rangle>")
   where
-  wr: "\<langle>(m,P)\<rangle> -t,W x v\<rightarrow> \<langle>(m,bufapp P x (PW v))\<rangle>" |
-  rd: "get m (P x) x = v \<Longrightarrow> \<langle>(m,P)\<rangle> -t,R x v\<rightarrow> \<langle>(m,P)\<rangle>" |
-  mf: "\<forall>y. PFO t \<notin> set (P y) \<Longrightarrow> \<langle>(m,P)\<rangle> -t,MF\<rightarrow> \<langle>(m,P)\<rangle>" |
-  fl: "P x = [] \<Longrightarrow> \<langle>(m,P)\<rangle> -t,FL x\<rightarrow> \<langle>(m,P)\<rangle>" |
-  fo: "\<langle>(m,P)\<rangle> -t,FO x\<rightarrow> \<langle>(m,bufapp P x (PFO t))\<rangle>" 
+  wr: "\<langle>m\<rangle> -t,W x v\<rightarrow> \<langle>m\<lbrakk>x \<^sub>@= PW v\<rbrakk>\<rangle>" |
+  rd: "get m x = v \<Longrightarrow> \<langle>m\<rangle> -t,R x v\<rightarrow> \<langle>m\<rangle>" |
+  mf: "\<forall>y. PFO t \<notin> set (buffers m y) \<Longrightarrow> \<langle>m\<rangle> -t,MF\<rightarrow> \<langle>m\<rangle>" |
+  fl: "buffers m x = [] \<Longrightarrow> \<langle>m\<rangle> -t,FL x\<rightarrow> \<langle>m\<rangle>" |
+  fo: "\<langle>m\<rangle> -t,FO x\<rightarrow> \<langle>m\<lbrakk>x \<^sub>@= PFO t\<rbrakk>\<rangle>" |
+  rmw: "get m x = v\<^sub>R \<Longrightarrow> \<forall>y. PFO t \<notin> set (buffers m y) \<Longrightarrow> \<langle>m\<rangle> -t,RMW x v\<^sub>R v\<^sub>W\<rightarrow> \<langle>m\<lbrakk>x \<^sub>@= PW v\<^sub>W\<rbrakk>\<rangle>" |
+  rmf: "get m x = v\<^sub>R \<Longrightarrow> \<forall>y. PFO t \<notin> set (buffers m y) \<Longrightarrow> \<langle>m\<rangle> -t,RMF x v\<^sub>R\<rightarrow> \<langle>m\<rangle>"
+
+definition eval :: "'t \<times> ('a,'b) event \<Rightarrow> ('a,'t,'b) state rel"
+  where "eval a = {(m,m'). \<langle>m\<rangle> -fst a,snd a\<rightarrow> \<langle>m'\<rangle>}"
+
+lemma step_det:
+  assumes "\<langle>m\<rangle> -t,\<alpha>\<rightarrow> \<langle>m'\<rangle>"
+  assumes "\<langle>m\<rangle> -t,\<alpha>\<rightarrow> \<langle>m''\<rangle>"
+  shows "m' = m''"
+  using assms by (induct) (auto elim: step.cases)
+
+lemma eval_det:
+  assumes "(m,m') \<in> eval \<alpha>"
+  assumes "(m,m'') \<in> eval \<alpha>"
+  shows "m' = m''"
+  using assms by (auto simp: eval_def intro: step_det)
+
+section \<open>Persistent Environment Steps\<close>
 
 inductive env :: "('a,'t,'b) state \<Rightarrow> ('a,'t,'b) state \<Rightarrow> bool"
   ("\<langle>_\<rangle> -e\<rightarrow> \<langle>_\<rangle>")
   where
-  pwr: "P x = (PW v)#p \<Longrightarrow> \<langle>(m,P)\<rangle> -e\<rightarrow> \<langle>(m(x := v),P(x := p))\<rangle>" |
-  pfo: "P x = (PFO t)#p \<Longrightarrow> \<langle>(m,P)\<rangle> -e\<rightarrow> \<langle>(m,P(x := p))\<rangle>"
+  pwr: "buffers m x = (PW v)#p \<Longrightarrow> \<langle>m\<rangle> -e\<rightarrow> \<langle>m\<lbrakk>x \<^sub>p= v\<rbrakk>\<lbrakk>x \<^sub>b= p\<rbrakk>\<rangle>" |
+  pfo: "buffers m x = (PFO t)#p \<Longrightarrow> \<langle>m\<rangle> -e\<rightarrow> \<langle>m\<lbrakk>x \<^sub>b= p\<rbrakk>\<rangle>"
+
+lemma pwrI [intro]:
+  assumes "buffers m x = (PW v)#p"
+  assumes "m' = m\<lbrakk>x \<^sub>p= v\<rbrakk>\<lbrakk>x \<^sub>b= p\<rbrakk>"
+  shows "\<langle>m\<rangle> -e\<rightarrow> \<langle>m'\<rangle>"
+  using env.intros(1) assms by metis
+
+lemma pfoI [intro]:
+  assumes "buffers m x = (PFO t)#p"
+  assumes "m' = m\<lbrakk>x \<^sub>b= p\<rbrakk>"
+  shows "\<langle>m\<rangle> -e\<rightarrow> \<langle>m'\<rangle>"
+  using env.intros(2) assms by metis
 
 inductive trace :: "('a,'t,'b) state \<Rightarrow> ('t \<times> ('a,'b) event) list \<Rightarrow> ('a,'t,'b) state \<Rightarrow> bool"
   where
@@ -64,500 +194,827 @@ inductive trace :: "('a,'t,'b) state \<Rightarrow> ('t \<times> ('a,'b) event) l
   step: "\<langle>m\<rangle> -thr,a\<rightarrow> \<langle>m'\<rangle> \<Longrightarrow> trace m' t m'' \<Longrightarrow> trace m ((thr,a)#t) m''" |
   env:  "\<langle>m\<rangle> -e\<rightarrow> \<langle>m'\<rangle> \<Longrightarrow> trace m' t m'' \<Longrightarrow> trace m t m''"
 
-lemma view_empty:
-  assumes "(snd m) x = []"
-  shows "view m x = (fst m) x"
-  using assms unfolding view_def by auto
+subsection \<open>Persistent Properties\<close>
 
-lemma view_now:
-  assumes "last_write ((snd m) x) = None"
-  shows "view m x = (fst m) x"
-  using assms unfolding view_def by auto
-
-lemma env_empty:
+lemma env_get [simp]:
   assumes "env m m'"
-  assumes "(snd m) x = []"
-  shows "(snd m') x = []"
-  using assms by (induct) auto
+  shows "get m x = get m' x"
+  using assms by cases (auto simp: get_def split: option.splits pevent.splits)
 
-lemma env_now:
-  assumes "env m m'"
-  assumes "last_write ((snd m) x) = None"
-  shows "last_write ((snd m') x) = None"
-  using assms 
+lemma envt_get [simp]:
+  assumes "env\<^sup>*\<^sup>* m m'"
+  shows "get m x = get m' x"
+  using assms
 proof (induct)
-  case (pwr P x v p m)
-  then show ?case
-    by (auto split: option.splits)
-next
-  case (pfo P x t p m)
+  case base
   then show ?case by auto
+next
+  case (step y z)
+  then show ?case using env_get by metis
 qed
 
-lemma env_now_eq:
-  assumes "env m m'"
-  assumes "last_write ((snd m) x) = None"
-  shows "fst m x = fst m' x"
-  using assms 
-proof (induct)
-  case (pwr P x v p m)
-  then show ?case
-    by (auto split: option.splits)
+lemma env_pers_setE:
+  assumes "env (m\<^sub>1\<lbrakk>x \<^sub>p= v\<rbrakk>) m\<^sub>2"
+  obtains (orth) m\<^sub>3 where "env m\<^sub>1 m\<^sub>3" "m\<^sub>2 = m\<^sub>3\<lbrakk>x \<^sub>p= v\<rbrakk>" |
+          (wr) v' l where "m\<^sub>2 = m\<^sub>1\<lbrakk>x \<^sub>p= v'\<rbrakk>\<lbrakk>x \<^sub>b= l\<rbrakk>" "buffers m\<^sub>1 x = (PW v')#l"
+  using assms
+proof cases
+  case (pwr y v' p)
+  have e: "\<langle>m\<^sub>1\<rangle> -e\<rightarrow> \<langle>m\<^sub>1\<lbrakk>y \<^sub>p= v'\<rbrakk>\<lbrakk>y \<^sub>b= p\<rbrakk>\<rangle>" using pwr by (auto intro: env.pwr)
+  then show ?thesis
+  proof (cases "x = y")
+    case True
+    then show ?thesis using pwr wr by auto
+  next
+    case False
+    then show ?thesis using pwr orth[OF e] by (simp add: fun_upd_twist)
+  qed
 next
-  case (pfo P x t p m)
-  then show ?case by auto
+  case (pfo y t p)
+  then show ?thesis using orth[of "m\<^sub>1\<lbrakk>y \<^sub>b= p\<rbrakk>"] by (auto intro: env.pfo)
 qed
 
-lemma env_view:
-  assumes "env m m'"
-  shows "view m x = view m' x"
-  using assms 
-proof (induct)
-  case (pwr P x v p m)
-  then show ?case by (auto simp: view_def split: option.splits)
-next
-  case (pfo P x t p m)
-  then show ?case by (auto simp: view_def split: option.splits)
-qed
+subsection \<open>Buffer Properties\<close>
 
 lemma env_buffers:
   assumes "env m m'"
-  shows "set (buffers m' x) \<subseteq> set (buffers m x)"
+  obtains pre where "buffers m x = pre @ buffers m' x"
   using assms 
-proof (induct)
-  case (pwr P x v p m)
-  then show ?case by (auto simp: view_def split: option.splits)
+proof cases
+  case (pwr y v p)
+  then show ?thesis using that by (cases "x = y") auto
 next
-  case (pfo P x t p m)
-  then show ?case by (auto simp: view_def split: option.splits)
+  case (pfo y t p)
+  then show ?thesis using that by (cases "x = y") auto
 qed
 
-
-lemma envt_empty:
-  assumes "env\<^sup>*\<^sup>* m m'"
-  assumes "(snd m) x = []"
-  shows "(snd m') x = []"
-  using assms
-proof (induct)
-  case base
-  then show ?case by auto
-next
-  case (step y z)
-  then show ?case using env_empty by fast
-qed
-
-lemma envt_now:
-  assumes "env\<^sup>*\<^sup>* m m'"
-  assumes "last_write ((snd m) x) = None"
-  shows "last_write ((snd m') x) = None"
-  using assms
-proof (induct)
-  case base
-  then show ?case by auto
-next
-  case (step y z)
-  then show ?case using env_now by fastforce
-qed
-
-lemma envt_now_eq:
-  assumes "env\<^sup>*\<^sup>* m m'"
-  assumes "last_write ((snd m) x) = None"
-  shows "fst m x = fst m' x"
-  using assms
-proof (induct)
-  case base
-  then show ?case by auto
-next
-  case (step y z)
-  then show ?case using env_now_eq envt_now by metis
-qed
-
-lemma envt_view:
-  assumes "env\<^sup>*\<^sup>* m m'"
-  shows "view m x = view m' x"
-  using assms
-proof (induct)
-  case base
-  then show ?case by auto
-next
-  case (step y z)
-  then show ?case using env_view by metis
-qed
+lemma env_buffer_empty:
+  assumes "env m m'"
+  assumes "buffers m x = []"
+  shows "buffers m' x = []"
+  using assms env_buffers
+  by (metis Nil_is_append_conv)
 
 lemma envt_buffers:
   assumes "env\<^sup>*\<^sup>* m m'"
-  shows "set (buffers m' x) \<subseteq> set (buffers m x)"
+  obtains pre where "buffers m x = pre @ buffers m' x"
   using assms
 proof (induct)
   case base
   then show ?case by auto
 next
   case (step y z)
-  then show ?case using env_buffers
-    by (metis (no_types, lifting) dual_order.trans)
+  then show ?case using env_buffers by (metis append.assoc)
 qed
 
-lemma [simp]:
-  assumes "x \<noteq> y"
-  shows "(bufapp P x e)(y := p) = bufapp (P(y := p)) x e"
-  using assms unfolding bufapp_def by auto
+lemma envt_buffer_empty:
+  assumes "env\<^sup>*\<^sup>* m m'"
+  assumes "buffers m x = []"
+  shows "buffers m' x = []"
+  using assms by (auto elim!: envt_buffers[where x = x])
 
-lemma [simp]:
-  shows "(bufapp P x e)(x := p) = P ( x:= p)"
-  unfolding bufapp_def by auto
+lemma envt_buffer_subset:
+  assumes "env\<^sup>*\<^sup>* m m'"
+  shows "set (buffers m' x) \<subseteq> set (buffers m x)"
+  using assms by (auto elim!: envt_buffers[where x = x])
 
-lemma [simp]:
-  assumes "x \<noteq> y"
-  shows "bufapp P\<^sub>1 x e y = P\<^sub>1 y"
-  using assms unfolding bufapp_def by auto
+subsubsection \<open>Introduction\<close>
 
-lemma [simp]:
-  shows "bufapp P\<^sub>1 x e x = P\<^sub>1 x @ [e]"
-  unfolding bufapp_def by auto
-
-lemma pre_postE:
-  assumes "A @ [e] = s # B"
-  obtains (empty) "A = []" "B = []" "e = s" |
-          (mid) l where "A = s # l" "B = l @ [e]"
+lemma env_buffer_appI:
+  assumes "env m m'"
+  shows "env (m\<lbrakk>x \<^sub>@= b\<rbrakk>) (m'\<lbrakk>x \<^sub>@= b\<rbrakk>)"
   using assms
-proof (induct A arbitrary: s B)
-  case Nil
-  then show ?case by auto
+proof cases
+  case (pwr y v p)
+  thus ?thesis by (cases "x = y") (auto intro!: pwrI[where x=y] simp add: fun_upd_twist)
 next
-  case (Cons a A)
-  hence [simp]: "a = s"  "B = A @ [e]" by auto
+  case (pfo y t p)
+  thus ?thesis by (cases "x = y") (auto intro!: pfoI[where x=y] simp add: fun_upd_twist)
+qed
 
-  show ?case
-  proof (cases "A = []")
-    case True
-    then show ?thesis using Cons by auto
+lemma envt_buffer_appI:
+  assumes "env\<^sup>*\<^sup>* m m'"
+  shows "env\<^sup>*\<^sup>* (m\<lbrakk>x \<^sub>@= b\<rbrakk>) (m'\<lbrakk>x \<^sub>@= b\<rbrakk>)"
+  using assms
+proof induct
+  case base
+  thus ?case by auto
+next
+  case (step y z)
+  thus ?case by (blast intro: env_buffer_appI rtranclp.rtrancl_into_rtrancl)
+qed
+
+lemma envt_full_evalI:
+  shows "env\<^sup>*\<^sup>* (m\<lbrakk>x \<^sub>@= PW v\<rbrakk>) (m\<lbrakk>x \<^sub>p= v\<rbrakk>\<lbrakk>x \<^sub>b= []\<rbrakk>)"
+proof (induct "buffers m x" arbitrary: m)
+  case Nil
+  hence "env (m\<lbrakk>x \<^sub>@= PW v\<rbrakk>) (m\<lbrakk>x \<^sub>p= v\<rbrakk>\<lbrakk>x \<^sub>b= []\<rbrakk>)" by auto
+  then show ?case by blast
+next
+  case (Cons pe p)
+  then show ?case  
+  proof (cases pe)
+    case (PFO t)
+    hence "env (m\<lbrakk>x \<^sub>@= PW v\<rbrakk>) (m\<lbrakk>x \<^sub>b= p @ [PW v]\<rbrakk>)" using Cons(2) by (intro pfoI[where t=t]) auto
+    then show ?thesis using Cons(1)[of "m\<lbrakk>x \<^sub>b= p\<rbrakk>"] by auto
   next
-    case False
-    then obtain a' A' where "A = a'#A'" by (cases A, auto)
-    hence a: "A @ [e] = a' # (A' @ [e])" by auto
-
-    show ?thesis
-    proof (rule Cons(1)[OF _ _ a], goal_cases)
-      case 1
-      then show ?case by auto
-    next
-      case (2 l)
-      then show ?case using Cons(3) by auto
-    qed
+    case (PW v')
+    hence "env (m\<lbrakk>x \<^sub>@= PW v\<rbrakk>) (m\<lbrakk>x \<^sub>p= v'\<rbrakk>\<lbrakk>x \<^sub>b= p @ [PW v]\<rbrakk>)" using Cons(2) by (intro pwrI) auto
+    then show ?thesis using Cons(1)[of "m\<lbrakk>x \<^sub>p= v'\<rbrakk>\<lbrakk>x \<^sub>b= p\<rbrakk>"] by auto
   qed
 qed
 
-lemma pre_postE':
-  assumes "s # B = A @ [e]"
-  obtains (empty) "A = []" "B = []" "e = s" |
-          (mid) l where "A = s # l" "B = l @ [e]"
-  using assms
-  using pre_postE by metis
+lemma envt_buffer_app_evalI:
+  assumes "env\<^sup>*\<^sup>* m m'"
+  shows "env\<^sup>*\<^sup>* (m\<lbrakk>x \<^sub>@= PW v\<rbrakk>) (m'\<lbrakk>x \<^sub>p= v\<rbrakk>\<lbrakk>x \<^sub>b= []\<rbrakk>)"
+  using envt_buffer_appI[OF assms] envt_full_evalI by (metis (mono_tags) rtranclp_trans)
 
+subsubsection \<open>Elimination\<close>
 
-lemma env_bufappE:
-  assumes "env (m\<^sub>1, bufapp P\<^sub>1 x e) (m\<^sub>2, P\<^sub>2)"
-  obtains (orth) P\<^sub>3 where "env (m\<^sub>1, P\<^sub>1) (m\<^sub>2, P\<^sub>3)" "P\<^sub>2 = bufapp P\<^sub>3 x e" |
-          (wr) v where "e = PW v" "m\<^sub>2 = m\<^sub>1 (x := v)" "P\<^sub>2 = P\<^sub>1" "P\<^sub>1 x = []" |
-          (fo) v where "e = PFO v" "m\<^sub>2 = m\<^sub>1" "P\<^sub>2 = P\<^sub>1" "P\<^sub>1 x = []"
+lemma env_buffer_appE:
+  assumes "env (m\<^sub>1\<lbrakk>x \<^sub>@= e\<rbrakk>) m\<^sub>2"
+  obtains (orth) m\<^sub>3 where "env m\<^sub>1 m\<^sub>3" "m\<^sub>2 = m\<^sub>3\<lbrakk>x \<^sub>@= e\<rbrakk>" |
+          (wr) v where "e = PW v" "m\<^sub>2 = m\<^sub>1\<lbrakk>x \<^sub>p= v\<rbrakk>" "buffers m\<^sub>1 x = []" |
+          (fo) v where "e = PFO v" "m\<^sub>2 = m\<^sub>1" "buffers m\<^sub>1 x = []"
   using assms
 proof cases
   case (pwr y v p)
   then show ?thesis
   proof (cases "x = y")
     case True
-    then show ?thesis
-    proof (cases "P\<^sub>1 x")
-      case Nil
-      then show ?thesis using True wr pwr apply auto by force
+    hence "buffers m\<^sub>1 y @ [e] = PW v # p" using pwr by auto
+    then show ?thesis 
+    proof (cases rule: post_preE)
+      case empty
+      then show ?thesis using wr pwr True by auto
     next
-      case (Cons a list)
-      then show ?thesis
-        using True orth[of "P\<^sub>1(y := list)"] pwr
-        by (auto simp: bufapp_def intro: env.intros)
+      case (mid l)
+      then show ?thesis using orth[of "m\<^sub>1\<lbrakk>y \<^sub>p= v\<rbrakk>\<lbrakk>y \<^sub>b= l\<rbrakk>"] pwr True by auto
     qed
   next
     case False
-    then show ?thesis using pwr orth[of "P\<^sub>1(y := p)"] by (auto intro: env.intros)     
+    then show ?thesis using pwr
+      by (intro orth[of "m\<^sub>1\<lbrakk>y \<^sub>p= v\<rbrakk>\<lbrakk>y \<^sub>b= p\<rbrakk>"] pwrI) (auto simp: fun_upd_twist)
   qed
 next
   case (pfo y t p)
   then show ?thesis
   proof (cases "x = y")
     case True
-    then show ?thesis
-    proof (cases "P\<^sub>1 x")
-      case Nil
-      then show ?thesis using True fo pfo apply auto by force
+    hence "buffers m\<^sub>1 y @ [e] = PFO t # p" using pfo by auto
+    then show ?thesis 
+    proof (cases rule: post_preE)
+      case empty
+      then show ?thesis using fo pfo True by auto
     next
-    next
-      case (Cons a list)
-      then show ?thesis
-        using True orth[of "P\<^sub>1(y := list)"] pfo
-        by (auto simp: bufapp_def intro: env.intros)
+      case (mid l)
+      then show ?thesis using orth[of "m\<^sub>1\<lbrakk>y \<^sub>b= l\<rbrakk>"] pfo True by auto
     qed
   next
     case False
-    then show ?thesis using pfo orth[of "P\<^sub>1(y := p)"] by (auto intro: env.intros)     
+    then show ?thesis using pfo
+      by (intro orth[of "m\<^sub>1\<lbrakk>y \<^sub>b= p\<rbrakk>"] pfoI) (auto simp: fun_upd_twist)
   qed
 qed
 
-(* 
-  x got written, how?
-    
-*)
-
-lemma bufappE:
-  assumes "env\<^sup>*\<^sup>* (m\<^sub>1, bufapp P\<^sub>1 x e) (m\<^sub>2, P\<^sub>2)"
-  obtains (orth) P\<^sub>3 where "env\<^sup>*\<^sup>* (m\<^sub>1, P\<^sub>1) (m\<^sub>2,P\<^sub>3)" "P\<^sub>2 = bufapp P\<^sub>3 x e" |
-          (wr) m\<^sub>3 v where "e = PW v" "env\<^sup>*\<^sup>* (m\<^sub>1, P\<^sub>1) (m\<^sub>3, P\<^sub>2)" "m\<^sub>2 = m\<^sub>3 (x := v)" "P\<^sub>2 x = []" |
-          (fo) v where "e = PFO v" "env\<^sup>*\<^sup>* (m\<^sub>1, P\<^sub>1) (m\<^sub>2, P\<^sub>2)" "P\<^sub>2 x = []" 
+lemma envt_buffer_appE:
+  assumes "env\<^sup>*\<^sup>* (m\<^sub>1\<lbrakk>x \<^sub>@= e\<rbrakk>) m\<^sub>2"
+  obtains (orth) m\<^sub>3 where "env\<^sup>*\<^sup>* m\<^sub>1 m\<^sub>3" "m\<^sub>2 = m\<^sub>3\<lbrakk>x \<^sub>@= e\<rbrakk>" |
+          (pwr) m\<^sub>3 v where "e = PW v" "env\<^sup>*\<^sup>* m\<^sub>1 m\<^sub>3" "m\<^sub>2 = m\<^sub>3\<lbrakk>x \<^sub>p= v\<rbrakk>" "buffers m\<^sub>2 x = []" |
+          (pfo) v where "e = PFO v" "env\<^sup>*\<^sup>* m\<^sub>1 m\<^sub>2" "buffers m\<^sub>2 x = []" 
   using assms
-proof (induct "(m\<^sub>1,bufapp P\<^sub>1 x e)" "(m\<^sub>2,P\<^sub>2)" arbitrary: m\<^sub>2 P\<^sub>2)
+proof (induct "m\<^sub>1\<lbrakk>x \<^sub>@= e\<rbrakk>" m\<^sub>2)
   case rtrancl_refl
   then show ?case by blast
 next
-  case (rtrancl_into_rtrancl b)
-  obtain m' P' where b: "b = (m',P')" by (cases b) 
-  then show ?case
+  case (rtrancl_into_rtrancl m\<^sub>3 m\<^sub>4)
+  show ?case
   proof (rule rtrancl_into_rtrancl(2), goal_cases)
-    case (1 P\<^sub>3)
-    hence "env (m', bufapp P\<^sub>3 x e) (m\<^sub>2, P\<^sub>2)" using rtrancl_into_rtrancl(3) unfolding b by auto
+    case (1 m\<^sub>5)
+    hence "env (m\<^sub>5\<lbrakk>x \<^sub>@= e\<rbrakk>) m\<^sub>4" using rtrancl_into_rtrancl(3) by simp
     then show ?case
-    proof (cases rule: env_bufappE)
-      case (orth P\<^sub>4)
-      then show ?thesis using 1 rtrancl_into_rtrancl(4)
-        by (metis rtranclp.rtrancl_into_rtrancl) 
+    proof (cases rule: env_buffer_appE)
+      case (orth m\<^sub>3')
+      then show ?thesis using rtrancl_into_rtrancl(4) 1(1) 
+        by (blast intro: rtranclp.rtrancl_into_rtrancl)
     next
       case (wr v)
-      then show ?thesis using 1 rtrancl_into_rtrancl(5) by blast
+      then show ?thesis using 1 rtrancl_into_rtrancl(5) by simp
     next
       case (fo v)
-      then show ?thesis using 1  rtrancl_into_rtrancl(6) by blast
+      then show ?thesis using 1 rtrancl_into_rtrancl(6) by simp
     qed
   next
-    case (2 v m\<^sub>3)
-    obtain m\<^sub>4 where "\<langle>(m\<^sub>3, P')\<rangle> -e\<rightarrow> \<langle>(m\<^sub>4, P\<^sub>2)\<rangle>" "m\<^sub>2 = m\<^sub>4(x := v)" "P\<^sub>2 x = []"
-      using rtrancl_into_rtrancl(3) 2(4) unfolding b 2(3)
-    proof (cases rule: env.cases)
-      case (pwr y v' p)
-      then show ?thesis using 2(4)  
-        apply (cases "x = y")
-        apply (auto intro: that)
-        using that[of "m\<^sub>3( y := v')"]
-        using env.intros(1)
-        by fastforce
+    case (2 v m\<^sub>5)
+    show ?case using rtrancl_into_rtrancl(3) unfolding 2
+    proof (cases rule: env_pers_setE)
+      case (orth m\<^sub>6)
+      then show ?thesis using 2 rtrancl_into_rtrancl(3,5)
+        by (blast intro: env_buffer_empty rtranclp.rtrancl_into_rtrancl)
     next
-      case (pfo y t p)
-      then show ?thesis using 2(4)
-        apply (cases "x = y")
-        apply (auto intro: that)
-        using that[of "m\<^sub>3"]
-        using env.intros(2)
-        by fastforce
+      case (wr v' l)
+      then show ?thesis using 2 by auto
     qed
-
-    then show ?case using 2 rtrancl_into_rtrancl(3) rtrancl_into_rtrancl(5)[of v m\<^sub>4] unfolding b 
-      by (meson rtranclp.rtrancl_into_rtrancl)
   next
     case (3 v)
-    then show ?case using 3 rtrancl_into_rtrancl(3) rtrancl_into_rtrancl(6)[of ] unfolding b
-      by (metis env_empty rtranclp.rtrancl_into_rtrancl snd_conv)
+    then show ?case using rtrancl_into_rtrancl(3,6) 
+      by (metis env_buffer_empty rtranclp.rtrancl_into_rtrancl)
+  qed
+qed
+
+lemma simple:
+  "m\<lbrakk>x \<^sub>b= p\<rbrakk>\<lbrakk>x \<^sub>b= q\<rbrakk>\<lbrakk>x \<^sub>p= f\<rbrakk> = m\<lbrakk>x \<^sub>b= q\<rbrakk>\<lbrakk>x \<^sub>p= f\<rbrakk>"
+  by (auto)
+
+lemma simple2:
+  "(m\<lbrakk>x \<^sub>p= a\<rbrakk>\<lbrakk>y \<^sub>b= b\<rbrakk>\<lbrakk>x \<^sub>p= c\<rbrakk>) = (m\<lbrakk>y \<^sub>b= b\<rbrakk>\<lbrakk>x \<^sub>p= c\<rbrakk>)"
+  by auto
+
+lemma flush_x:
+  shows "env\<^sup>*\<^sup>* m (m\<lbrakk>x \<^sub>b= []\<rbrakk>\<lbrakk>x \<^sub>p= get m x\<rbrakk>)"
+proof (induct "buffers m x" arbitrary: m)
+  case Nil
+  hence "m\<lbrakk>x \<^sub>b= []\<rbrakk>\<lbrakk>x \<^sub>p= get m x\<rbrakk> = m" by auto
+  then show ?case by (metis rtranclp.rtrancl_refl)
+next
+  case (Cons a p)
+  hence t: "buffers m x = a # p" by auto
+
+  then show ?case
+  proof (cases a)
+    case (PFO x1)
+    hence "env\<^sup>*\<^sup>* (m\<lbrakk>x \<^sub>b= p\<rbrakk>) (m\<lbrakk>x \<^sub>b= p\<rbrakk>\<lbrakk>x \<^sub>b= []\<rbrakk>\<lbrakk>x \<^sub>p= get (m\<lbrakk>x \<^sub>b= p\<rbrakk>) x\<rbrakk>)"
+      using Cons 
+      by (metis (mono_tags, lifting) fun_upd_same select_convs(2) surjective update_convs(1,2))
+    moreover have e: "\<langle>m\<rangle> -e\<rightarrow> \<langle>m\<lbrakk>x \<^sub>b= p\<rbrakk>\<rangle>" using PFO env.pfo t by blast
+    ultimately show ?thesis  unfolding simple 
+      by (smt (verit, best) converse_rtranclp_into_rtranclp env_get surjective update_convs(1))
+
+  next
+    case (PW v)
+    let ?m="m\<lbrakk>x \<^sub>p= v\<rbrakk>\<lbrakk>x \<^sub>b= p\<rbrakk>"
+    have "env\<^sup>*\<^sup>* ?m (?m\<lbrakk>x \<^sub>b= []\<rbrakk>\<lbrakk>x \<^sub>p= get ?m x\<rbrakk>)"
+      using Cons PW
+      by (smt (verit, best) fun_upd_same select_convs(2) surjective update_convs(1,2))
+    moreover have e: "\<langle>m\<rangle> -e\<rightarrow> \<langle>m\<lbrakk>x \<^sub>p= v\<rbrakk>\<lbrakk>x \<^sub>b= p\<rbrakk>\<rangle>" using PW env.pwr t by blast
+    moreover have "get (m\<lbrakk>x \<^sub>p= v\<rbrakk>\<lbrakk>x \<^sub>b= p\<rbrakk>) x = get m x"
+      unfolding get_def t PW 
+      by (auto split: option.splits pevent.splits)
+    ultimately show ?thesis unfolding simple simple2 
+      by (metis (mono_tags, lifting) converse_rtranclp_into_rtranclp surjective update_convs(1))
   qed
 qed
 
 
-lemma last_write_app [simp]:
-  "last_write (a @ [PW v]) = Some v"
-proof (induct a)
-  case Nil
-  then show ?case by auto
-next
-  case (Cons a1 a2)
-  then show ?case by (cases a1; auto)
-qed
-
-lemma view_bufapp [simp]:
-  shows "view (a,bufapp b x (PW v)) = (view (a, b))(x := v)"
-  unfolding view_def bufapp_def by auto
-
-
-lemma view_empty_buf_upd [simp]:
-  assumes "b x = []"
-  shows "(view (a,b))(x := v) = (view (a(x := v), b))"
-  using assms unfolding view_def fun_eq_iff by (auto  split: option.splits)
 
 section \<open>Predicate Language\<close>
 
-text \<open>Predicate abstraction to simplify specification\<close>
-type_synonym ('a,'b) pred = "(('a,'b) m \<times> ('a,'b) m \<times> ('a,'b) m) set"
+type_synonym ('a,'t) ord = "'a \<Rightarrow> 't \<Rightarrow> bool"
 
-definition contains :: "'a list \<Rightarrow> ('a) \<Rightarrow> bool"
-  where "contains l f \<equiv> f \<in> set l"
+text \<open>Predicate abstraction to simplify specification, consisting of: 
+      (volatile memory, persistent memory, memory after an mfence)\<close>
+type_synonym ('a,'b,'t) pred = "(('a,'b) m \<times> ('a,'b) m \<times> ('a,'b) m) set"
+type_synonym ('a,'b,'t) prel = "(('a,'b) m \<times> ('a,'b) m \<times> ('a,'b) m) rel"
 
-fun isPFO
-  where "isPFO (PFO _) = True" | "isPFO _ = False"
+subsection \<open>pre_fo\<close>
 
-fun foslice :: "'t \<Rightarrow> ('t,'b) pevent list \<Rightarrow> 'b option"
+text \<open>Find a write before a PFO event in a buffer, returning None if there aren't any\<close>
+fun pre_fo :: "'t \<Rightarrow> ('t,'b) pevent list \<Rightarrow> 'b option"
   where 
-    "foslice t [] = None" |
-    "foslice t (PFO _#xs) = (if \<not>(contains xs (PFO t)) then None else foslice t xs)" |
-    "foslice t (PW x#PFO t'#xs) = (if t' = t \<and> \<not>(contains xs (PFO t)) then Some x else foslice t (PW x#xs) )" |
-    "foslice t (PW x#xs) = foslice t xs"
+    "pre_fo t [] = None" |
+    "pre_fo t (PFO _#xs) = (if PFO t \<in> set xs then pre_fo t xs else None)" |
+    "pre_fo t (PW x#PFO s#xs) = (if s = t \<and> PFO t \<notin> set xs then Some x else pre_fo t (PW x#xs))" |
+    "pre_fo t (PW x#xs) = pre_fo t xs"
 
-definition foget :: "'t \<Rightarrow> ('a,'b) m \<times> ('a,'t,'b) pbuffers \<Rightarrow> ('a,'b) m"
-  where "foget t m a \<equiv> (case foslice t (buffers m a) of Some v \<Rightarrow> v | None \<Rightarrow> persistent m a)"
-
-definition sat :: "'t \<Rightarrow> ('a,'b) pred \<Rightarrow> ('a,'b) m \<times> ('a,'t,'b) pbuffers \<Rightarrow> bool"
-  where "sat t Q m \<equiv> \<forall>m'. env\<^sup>*\<^sup>* m m' \<longrightarrow> (view m', persistent m', foget t m') \<in> Q"
-
-fun wp :: "('a,'b) event \<Rightarrow> ('a,'b) pred \<Rightarrow> ('a,'b) pred"
-  where
-    "wp (W x v) Q = {(m,p,f). (m(x:=v),p,f) \<in> Q \<and> (m(x:=v),p(x:=v),f(x:=v)) \<in> Q }" |
-    "wp (R x v) Q = {(m,p,f). m x = v \<longrightarrow> (m,p,f) \<in> Q}" |
-    "wp (FL x) Q = {(m,p,f). m x = p x \<and> m x = f x \<longrightarrow> (m,p,f) \<in> Q}" |
-    "wp MF Q = {(m,p,f). p = f \<longrightarrow> (m,p,f) \<in> Q}" |
-    "wp (FO x) Q = {(m,p,f). (m,p,f(x := m x)) \<in> Q}"
-
-fun wpl :: "'t \<Rightarrow> ('t \<times> ('a,'b) event) list \<Rightarrow> ('a,'b) pred \<Rightarrow> ('a,'b) pred"
-  where
-    "wpl t [] A = A" |
-    "wpl t ((t',x)#xs) A = (if t = t' then wp x (wpl t xs A) else wpl t xs A)"
-
-lemma foget_empty:
-  "buffers m x = [] \<Longrightarrow> foget t m x = persistent m x"
-  unfolding foget_def by auto
-
-lemma [simp]:
-  "foslice t (p @ [PW v]) = foslice t p"
-  by (induct t "p" rule: foslice.induct) (auto simp: contains_def)
-
-lemma foget_bufapp [simp]:
-  shows "foget t (a,bufapp b x (PW v)) = (foget t (a, b))"
-  unfolding foget_def bufapp_def fun_eq_iff by (auto split: option.splits)
-
-lemma foget_empty_buf_upd [simp]:
-  assumes "b x = []"
-  shows "(foget t (a,b))(x := v) = (foget t (a(x := v), b))"
-  using assms unfolding foget_def fun_eq_iff by (auto  split: option.splits)
-
-lemma [simp]:
-  "last_write (p @ [PFO t]) = last_write p"
-proof (induct p)
-  case Nil
-  then show ?case by auto
-next
-  case (Cons a p)
-  then show ?case by (cases a) auto
-qed
-
-lemma [simp]:
-  "view (a, bufapp b x (PFO t)) = view (a, b)"
-  unfolding view_def bufapp_def fun_eq_iff by (auto split: option.splits)
-
-lemma [simp]:
-  "foslice t (l @ [PFO t]) = last_write l"
-proof (induct t "l@[PFO t]" arbitrary: l rule: foslice.induct )
-  case (1 t)
-  then show ?case by auto
-next
-  case (2 t uu xs)
-  then show ?case by (auto simp: contains_def elim!: pre_postE' split: option.splits)
-next
-  case (3 t x t' xs)
-  then show ?case by (auto simp: contains_def elim!: pre_postE' split: option.splits)
-next
-  case ("4_1" t x)
-  then show ?case by auto
-next
-  case ("4_2" t x vb va)
-  then show ?case by (auto elim!: pre_postE' split: option.splits)
-qed
-
-lemma [simp]:
-  "foget t (a, bufapp b x (PFO t)) x = view (a, b) x"
-  unfolding view_def foget_def bufapp_def by (auto split: option.splits)
-
-lemma [simp]:
-  "foget t (a, bufapp b x (PFO t)) = (foget t (a, b)) (x := view (a,b) x)"
-  unfolding view_def foget_def bufapp_def by (auto split: option.splits)
-
-lemma foslice_npfo:
+lemma pre_fo_no_pfo [simp]:
   assumes "PFO t \<notin> set l" 
-  shows "foslice t l = None"
-  using assms by (induct t l rule: foslice.induct) auto
+  shows "pre_fo t l = None"
+  using assms by (induct l rule: pre_fo.induct) auto
 
-lemma foget_npfo [simp]:
-  assumes "\<forall>y. PFO t \<notin> set (buffers m y)" 
-  shows "foget t m = fst m"
-  using assms unfolding foget_def fun_eq_iff 
-  apply (auto split: option.splits)
-  by (simp add: foslice_npfo)
+lemma pre_fo_no_pw [simp]:
+  assumes "\<forall>e \<in> set l. \<not> isPW e"
+  shows "pre_fo t l = None"
+  using assms by (induct l rule: pre_fo.induct) auto
 
-lemma wp_sound:
-  assumes "\<langle>m\<rangle> -t,a\<rightarrow> \<langle>m'\<rangle>" "sat t (wp a Q) m"
-  shows "sat t Q m'"
-  using assms
-proof (induct)
-  case (wr m P t x v)
-  then show ?case
-    apply auto
-    unfolding sat_def
-    apply auto
-    apply (elim bufappE)
-      apply (auto)
-    by fastforce
-next
-  case (rd m P x v t)
-  hence "view (m,P) x = v" by (auto simp: view_def)
-  then show ?case using rd(2) by (auto simp add: sat_def envt_view)
-next
-  case (mf t P m)
-  then show ?case
-    unfolding sat_def wp.simps
-    apply auto
-    using foget_npfo 
-    apply (subgoal_tac " \<forall>y. PFO t \<notin> set (buffers (a,b) y)")
-     apply (subgoal_tac "foget t  (a,b) = persistent  (a,b)")
-      apply auto[2]
-    using envt_buffers
-    by fastforce
-next
-  case (fl P x m t)
-  then show ?case
-    unfolding sat_def wp.simps
-    using view_empty envt_empty foget_empty
-    by (smt (verit, ccfv_SIG) case_prodD mem_Collect_eq snd_eqD)
-next
-  case (fo m P t x)
-  then show ?case
-    unfolding sat_def 
-    apply auto
-    apply (elim bufappE)
-      apply auto
-     apply (metis (no_types, opaque_lifting) foget_empty fun_upd_triv snd_conv view_empty)
-    done    
-qed
+lemma pre_fo_pfo [simp]:
+  "pre_fo t (l @ [PFO t]) = (case lastf isPW l of Some (PW v) \<Rightarrow> Some v | _ \<Rightarrow> None)"
+  by (induct "l@[PFO t]" arbitrary: l rule: pre_fo.induct)
+      (auto elim!: pre_postE split: option.splits pevent.splits)
+
+lemma pre_fo_pw [simp]:
+  "pre_fo t (l @ [PW v]) = pre_fo t l"
+  by (induct "l@[PW v]" arbitrary: l rule: pre_fo.induct)
+      (auto elim!: pre_postE split: option.splits)
+
+lemma pre_fo_other [simp]:
+  "s \<noteq> t \<Longrightarrow> pre_fo t (l @ [PFO s]) = pre_fo t l"
+  by (induct "l@[PFO t]" arbitrary: l rule: pre_fo.induct)
+      (auto elim!: pre_postE split: option.splits pevent.splits)
+
+subsection \<open>get for @{term PFO} effects\<close>
+
+text \<open>Persistent memory after an @{term MF} is evaluated\<close>
+definition get\<^sub>f :: "'t \<Rightarrow> ('a,'t,'b) state \<Rightarrow> ('a,'b) m"
+  where "get\<^sub>f t m a \<equiv> case pre_fo t (buffers m a) of Some v \<Rightarrow> v | None \<Rightarrow> persistent m a"
+
+lemma get\<^sub>f_no_pfo[simp]:
+  assumes "\<forall>y. PFO t \<notin> set (buffers m y)"
+  shows "get\<^sub>f t m = persistent m"
+  using assms by (auto simp: get\<^sub>f_def fun_eq_iff split: option.splits)
+
+lemma get\<^sub>f_no_pw[simp]:
+  assumes "\<forall>e \<in> set (buffers m x). \<not> isPW e"
+  shows "get\<^sub>f t m x = persistent m x"
+  using assms by (auto simp: get\<^sub>f_def fun_eq_iff split: option.splits pevent.splits)
+
+lemma get\<^sub>f_app_pfo [simp]:
+  "get\<^sub>f t (m\<lbrakk>x \<^sub>@= PFO t\<rbrakk>) = (get\<^sub>f t m)(x := get m x)"
+  by (auto simp: get_def fun_eq_iff get\<^sub>f_def split: option.splits pevent.splits)
+
+lemma [simp]:
+  assumes "\<forall>e \<in> set (buffers m x). \<not> isPW e"
+  shows "get\<^sub>f t (m\<lbrakk>x \<^sub>p= v\<rbrakk>) = (get\<^sub>f t m)(x := v)"
+  using assms by (auto simp: get\<^sub>f_def fun_eq_iff split: option.splits pevent.splits)
+
+lemma get\<^sub>f_app_simps [simp]:
+  "get\<^sub>f t (m\<lbrakk>x \<^sub>@= PW v\<rbrakk>) = (get\<^sub>f t m)"
+  by (auto simp: get_def get\<^sub>f_def fun_eq_iff split: option.splits pevent.splits)
+
+lemma [simp]:
+  "get\<^sub>f t m x = c \<Longrightarrow> (get\<^sub>f t m)(x := c) = get\<^sub>f t m"
+  by auto
+
+lemma [simp]:
+  "get\<^sub>f t (m\<lbrakk>x \<^sub>p= v\<rbrakk>\<lbrakk>x \<^sub>b= []\<rbrakk>) = (get\<^sub>f t m)(x := v)"
+  unfolding get\<^sub>f_def fun_eq_iff by (auto split: option.splits)
+
+lemma [simp]:
+  "s \<noteq> t \<Longrightarrow> get\<^sub>f s (m\<lbrakk>x \<^sub>@= PFO t\<rbrakk>) = get\<^sub>f s m"
+  by (auto simp: get\<^sub>f_def fun_eq_iff split: option.splits)
+
+subsection \<open>sat\<close>
+
+definition sat :: "'t \<Rightarrow> ('a,'b,'t) pred \<Rightarrow> ('a,'t,'b) state \<Rightarrow> bool"
+  where "sat t Q m \<equiv> \<forall>m'. env\<^sup>*\<^sup>* m m' \<longrightarrow> (get m', persistent m', get\<^sub>f t m') \<in> Q"
 
 lemma sat_env_stable:
   assumes "sat t Q m" "\<langle>m\<rangle> -e\<rightarrow> \<langle>m'\<rangle>"
   shows "sat t Q m'"
   using assms unfolding sat_def
   by (meson converse_rtranclp_into_rtranclp)
-  
-lemma wpl_sound:
-  assumes "trace m t m'" "sat thr (wpl t Q) m"
-  shows "sat thr Q m'"
+
+subsection \<open>wp\<close>
+
+fun wp :: "('a,'b) event \<Rightarrow> ('a,'b,'t) pred \<Rightarrow> ('a,'b,'t) pred"
+  where
+    "wp (W x v) Q = {(m,p,f). (m(x:=v),p,f) \<in> Q \<and> (m(x:=v),p(x:=v),f(x:=v)) \<in> Q}" |
+    "wp (R x v) Q = {(m,p,f). m x = v \<longrightarrow> (m,p,f) \<in> Q}" |
+    "wp (FL x) Q = {(m,p,f). (m,p(x := m x),f(x := m x)) \<in> Q}" |
+    "wp MF Q = {(m,p,f). (m,f,f) \<in> Q}" |
+    "wp (FO x) Q = {(m,p,f). (m,p,f(x := m x)) \<in> Q}" |
+    "wp (RMW x v\<^sub>R v\<^sub>W) Q = {(m,p,f). m x = v\<^sub>R \<longrightarrow> (m(x:=v\<^sub>W),f,f) \<in> Q \<and> (m(x:=v\<^sub>W),f(x:=v\<^sub>W),f(x:=v\<^sub>W)) \<in> Q}" |
+    "wp (RMF x v\<^sub>R) Q = {(m,p,f). m x = v\<^sub>R \<longrightarrow> (m,f,f) \<in> Q}"
+
+lemma wp_sound:
+  assumes "\<langle>m\<rangle> -t,a\<rightarrow> \<langle>m'\<rangle>" 
+  shows "sat t (wp a Q) m \<longrightarrow> sat t Q m'"
   using assms
+proof (cases)
+  case (wr x v)
+  thus ?thesis
+    apply (clarsimp simp: sat_def)
+    apply (elim envt_buffer_appE)
+    by auto
+next
+  case (rd x v)
+  thus ?thesis by (auto simp: sat_def)
+next
+  case mf
+  hence "\<forall>y m'. env\<^sup>*\<^sup>* m m' \<longrightarrow> PFO t \<notin> set (buffers m' y)" by (meson envt_buffer_subset in_mono)
+  thus ?thesis using mf by (auto simp: sat_def)
+next
+  case (fl x)
+  hence "\<forall>m'. env\<^sup>*\<^sup>* m m' \<longrightarrow> buffers m' x = []" using envt_buffer_empty by metis
+  thus ?thesis using fl by (auto simp: sat_def)
+next
+  case (fo x)
+  thus ?thesis by (auto elim!: envt_buffer_appE simp: sat_def)
+next
+  case (rmw x v\<^sub>R v\<^sub>W)
+  hence "\<forall>y m'. env\<^sup>*\<^sup>* m m' \<longrightarrow> PFO t \<notin> set (buffers m' y)" by (meson envt_buffer_subset in_mono)
+  then show ?thesis using rmw apply (clarsimp simp: sat_def)
+    apply (elim envt_buffer_appE)
+    by auto
+next
+  case (rmf x v\<^sub>R)
+  hence "\<forall>y m'. env\<^sup>*\<^sup>* m m' \<longrightarrow> PFO t \<notin> set (buffers m' y)" by (meson envt_buffer_subset in_mono)
+  then show ?thesis using rmf by (auto simp: sat_def)
+qed
+ 
+subsection \<open>Concurrency\<close>
+
+definition wpr
+  where "wpr r Q \<equiv> {(m,p,f). \<forall>m' p' f'. ((m,p,f),(m',p',f')) \<in> r \<longrightarrow>  (m',p',f') \<in> Q}"
+
+fun guar
+  where
+    "guar q (W x v) r = {(m,p,f). \<forall>s. ((m,p,s),(m(x := v),p,s)) \<in> r \<and> ((m,p,s),(m(x := v),p(x := v),s(x := v))) \<in> r}" |
+    "guar q (RMW x v\<^sub>R v\<^sub>W) r = {(m,p,f). m x = v\<^sub>R \<longrightarrow> (\<forall>s. ((m,p,s),(m(x := v\<^sub>W),p,s)) \<in> r \<and> ((m,p,s),(m(x := v\<^sub>W),p(x := v\<^sub>W),s(x := v\<^sub>W))) \<in> r)}" |
+    "guar q _ r = UNIV"
+
+fun beh
+  where
+    "beh (W x v) = ({((m,p,f,s),(m(x := v),p,f,s))| m p f s. True} \<union> {((m,p,f,s),(m(x := v),p(x := v),f(x := v),s(x := v))) | m p s f. True})" |
+    "beh (R x v) = {((m,p,f,s),(m,p,f,s))| m p f s. m x = v}" |
+    "beh (FL x)  = {((m,p,f,s),(m,p(x := m x),f(x := m x),s(x := m x)))| m p f s. True}" |
+    "beh MF      = {((m,p,f,s),(m,f,f,s))| m p f s. True}" |
+    "beh (FO x)  = {((m,p,f,s),(m,p,f(x := m x),s))|m p f s. True}" |
+    "beh (RMW x v\<^sub>R v\<^sub>W) = ({((m,p,f,s),(m(x := v\<^sub>W),f,f,s))| m p f s . m x = v\<^sub>R} \<union> {((m,p,f,s),(m(x := v\<^sub>W),p(x := v\<^sub>W),f(x := v\<^sub>W),s(x := v\<^sub>W))) | m p f s . m x = v\<^sub>R})" |
+    "beh (RMF x v\<^sub>R) = {((m,p,f,s),(m,f,f,s))| m p f s. m x = v\<^sub>R}" 
+
+lemma step_rw:
+  assumes "\<langle>m\<rangle> -t,x\<rightarrow> \<langle>m'\<rangle>"
+  assumes "persistent m' = persistent m''"
+  assumes "buffers m' = buffers m''"
+  assumes "more m' = more m''"
+  shows "\<langle>m\<rangle> -t,x\<rightarrow> \<langle>m''\<rangle>"
+  using assms equality by blast
+
+
+lemma wpr_sound:
+  assumes "\<langle>m\<rangle> -t,a\<rightarrow> \<langle>m'\<rangle>" "sat t (guar t a r) m" "s \<noteq> t"
+  assumes "sat s (wpr (r) Q) m" "trans (r)"
+  shows "sat s (wpr (r) Q) m'"
+  using assms
+proof (cases)
+  case (wr x v)
+  hence "\<forall>m'. env\<^sup>*\<^sup>* m m' \<longrightarrow> get m = get m'" by auto
+  then show ?thesis using assms wr
+    apply (clarsimp simp: sat_def wpr_def)
+    apply (elim envt_buffer_appE; simp)
+     apply (meson transD)
+    by (meson transD)
+next
+  case (rd x v)
+  hence "\<forall>m'. env\<^sup>*\<^sup>* m m' \<longrightarrow> get m = get m'" by auto
+  then show ?thesis using assms(4) rd 
+    by (clarsimp simp: sat_def wpr_def)
+next
+  case mf
+  hence "\<forall>m'. env\<^sup>*\<^sup>* m m' \<longrightarrow> get m = get m'" by auto
+  then show ?thesis using assms(4) mf 
+    by (clarsimp simp: sat_def wpr_def)
+next
+  case (fl x)
+  hence "\<forall>m'. env\<^sup>*\<^sup>* m m' \<longrightarrow> get m = get m'" by auto
+  then show ?thesis using assms(4) fl 
+    by (clarsimp simp: sat_def wpr_def)
+next
+  case (fo x)
+  hence "\<forall>m'. env\<^sup>*\<^sup>* m m' \<longrightarrow> get m = get m'" by auto
+  then show ?thesis using assms(3,4) fo 
+    apply (clarsimp simp: sat_def wpr_def)
+    by (elim envt_buffer_appE; simp)
+next
+  case (rmw x v\<^sub>R v\<^sub>W)
+  hence "\<forall>m'. env\<^sup>*\<^sup>* m m' \<longrightarrow> get m = get m'" by auto
+  then show ?thesis using assms rmw
+    apply (clarsimp simp: sat_def wpr_def)
+    apply (elim envt_buffer_appE; simp)
+     apply (meson transD)
+    by (meson transD)
+next                 
+  case (rmf x v\<^sub>R)
+  hence "\<forall>m'. env\<^sup>*\<^sup>* m m' \<longrightarrow> get m = get m'" by auto
+  then show ?thesis using assms(4) rmf 
+    by (clarsimp simp: sat_def wpr_def)
+qed
+
+lemma guar_mono:
+  assumes "r \<subseteq> g"
+  shows "guar t a r \<subseteq> guar t a g"
+  using assms by (cases a; clarsimp) blast+
+
+subsection \<open>wpl\<close>
+
+fun wpl :: "'t \<Rightarrow>  ('a,'b,'t) prel \<Rightarrow> ('a,'b,'t) prel \<Rightarrow> ('a,'b) event list \<Rightarrow> ('a,'b,'t) pred \<Rightarrow> ('a,'b,'t) pred"
+  where
+    "wpl t r g [] A = wpr r A" |
+    "wpl t r g (x#xs) A = wpr r (wp x (wpl t r g xs A) \<inter> guar t x g)"
+
+fun id_filter
+  where 
+    "id_filter t [] = []" |
+    "id_filter t ((s,e)#p) = (if t = s then e#(id_filter t p) else id_filter t p)"
+
+definition compat
+  where "compat r g \<equiv> \<forall>i j. i \<noteq> j \<longrightarrow> g i \<subseteq> r j"
+
+lemma wpr_pres:
+  assumes "sat s (wpr r Q) m" "refl r"
+  shows "sat s Q m"
+  using assms unfolding sat_def wpr_def
+  apply clarsimp
+  by (metis UNIV_I refl_on_def)
+
+lemma [simp]:
+  "sat t (P \<inter> Q) m = (sat t P m \<and> sat t Q m)"
+  unfolding sat_def by auto
+
+lemma sat_imp:
+  "sat t P m \<Longrightarrow> P \<subseteq> Q \<Longrightarrow> sat t Q m"
+  by (auto simp: sat_def)
+
+lemma wp_mono:
+  assumes "P \<subseteq> Q"
+  shows "wp a P \<subseteq> wp a Q"
+  using assms by (cases a) auto
+
+lemma wp_mono':
+  assumes "m \<in> wp a P"
+  assumes "P \<subseteq> Q"
+  shows "m \<in> wp a Q"
+  using assms by (cases a) auto
+
+lemma wpl_sound:
+  assumes "trace m ts m'" "\<forall>t. sat t (wpl t (r t) (g t) (id_filter t ts) (Q t)) m"
+  assumes compat: "compat r g" 
+  assumes refl: "\<forall>t. refl (r t) \<and> trans (r t)"
+  shows "\<forall>t. sat t (Q t) m'"
+  using assms(1,2)
 proof (induct arbitrary: Q)
   case (nil a)
-  then show ?case by auto
+  then show ?case
+    apply simp
+    using refl wpr_pres by metis
 next
-  case (step m u a m' t m'')
-  then show ?case using wp_sound by fastforce
+  case (step m t a m' ts m'')
+  have t: "sat t (wpl t (r t) (g t) (id_filter t ((t, a) # ts)) (Q t)) m" using step(4) by blast
+  hence g: "sat t (guar t a (g t)) m" 
+    apply simp
+    apply (drule wpr_pres, insert refl, blast)
+    by auto
+
+  show ?case 
+  proof (rule step(3), intro allI)
+    fix s 
+    have a: "sat s (wpl s (r s) (g s) (id_filter s ((t, a) # ts)) (Q s)) m" using step by auto
+    show "sat s (wpl s (r s) (g s) (id_filter s ts) (Q s)) m'"
+    proof (cases "s = t")
+      case True
+      then show ?thesis
+        using a step(1)
+        apply simp
+        by (drule wpr_pres, insert refl, blast) (simp add: wp_sound)
+    next
+      case False
+      hence "g t \<subseteq> r s" using assms by (auto simp: compat_def)
+      hence "guar t a (g t) \<subseteq> guar t a (r s)" by (rule guar_mono)
+      hence g: "sat t (guar t a (r s)) m"
+        using g sat_imp by meson
+
+      show ?thesis
+      proof (cases "id_filter s ts")
+        case Nil
+        then show ?thesis using refl False a wpr_sound[OF step(1) g False] by simp
+      next
+        case (Cons a list)
+        then show ?thesis using refl False a wpr_sound[OF step(1) g False] by simp
+      qed
+    qed
+  qed
 next
   case (env m m' t m'')
-  then show ?case using sat_env_stable by fastforce
+  then show ?case using sat_env_stable by metis
 qed
+
+definition interleave
+  where "interleave ts ts' \<equiv> \<forall>t. id_filter t ts = id_filter t ts'"    
+
+lemma interleave_nil:
+  "interleave [] []"
+  by (auto simp: interleave_def)
+
+lemma interleave_cons:
+  "interleave x y \<Longrightarrow> interleave (a#x) (a#y)"
+  by (cases a) (auto simp: interleave_def)
+
+lemma tenv_traceI:
+  assumes "env\<^sup>*\<^sup>* m m'" "trace m' ts m''"
+  shows "trace m ts m''"
+  using assms
+proof (induct)
+  case base
+  then show ?case by auto
+next
+  case (step y z)
+  then show ?case 
+    using env by blast 
+qed
+
+lemma sat_conj:
+  assumes "sat t P m" "sat t Q m"
+  shows "sat t (P \<inter> Q) m"
+  using assms by (auto simp: sat_def)
+
+lemma id_filter_remove_other [simp]: 
+  "s \<noteq> t \<Longrightarrow> id_filter s (remove1 (t, x) ts) = id_filter s ts"
+  by (induct ts) (auto split: if_splits)
+
+lemma id_filter_remove:
+  assumes "id_filter t ts = x#re"
+  shows "id_filter t (remove1 (t,x) ts) = re"
+  using assms
+proof (induct ts arbitrary: re)
+  case Nil
+  then show ?case by auto
+next
+  case (Cons a ts)
+  then show ?case by (cases a) auto
+qed
+
+lemma interleave_remove:
+  assumes "interleave (remove1 (t, x) ts) ts'"
+  assumes "id_filter t ts = x#p"
+  shows "interleave ts ((t,x)#ts')"
+  using assms
+  unfolding interleave_def
+  apply auto
+   prefer 2
+    apply (frule id_filter_remove_other[where ts=ts and x=x])
+   apply simp
+  apply (frule id_filter_remove)
+  apply simp
+  done
+
+subsection \<open>raise\<close>
+
+text \<open>Convert the predicate encoding into a minimal state\<close>
+definition raise
+  where "raise t v p f \<equiv> \<lparr> persistent = p , 
+                           buffers = \<lambda>x. (if p x \<noteq> f x then [PW (f x), PFO t] else []) @
+                                         (if v x \<noteq> f x then [PW (v x)] else []) \<rparr>"
+
+lemma [simp]:
+  "get (raise t v p f) = v"
+  by (auto simp: fun_eq_iff raise_def get_def)
+
+lemma [simp]:
+  "persistent (raise t v p f) = p"
+  by (auto simp: fun_eq_iff raise_def)
+
+lemma [simp]:
+  "get\<^sub>f t (raise t v p f) = f"
+  by (auto simp: fun_eq_iff raise_def get\<^sub>f_def contains_def)
+
+
+lemma sat_wprI':
+  assumes "\<And>m' m'' . env\<^sup>*\<^sup>* m m' \<longrightarrow> ((get m', persistent m', get\<^sub>f t m'),(get m'', persistent m'', get\<^sub>f t m'')) \<in> r \<longrightarrow> sat t Q m''"
+  shows "sat t (wpr r Q) m"
+  using assms unfolding sat_def wpr_def
+  apply auto
+  apply (subgoal_tac "((get m', persistent m', get\<^sub>f t m'), (get (raise t m'a p' f'), persistent  (raise t m'a p' f'), get\<^sub>f t  (raise t m'a p' f'))) \<in> r")
+  prefer 2
+   apply auto[1]
+  apply (subgoal_tac "(get (raise t m'a p' f'), persistent (raise t m'a p' f'), get\<^sub>f t (raise t m'a p' f')) \<in> Q")
+   apply simp
+  by blast
+
+
+
+
+section \<open>Completeness\<close>
+
+text \<open>
+Implication is sound but not complete for this encoding.
+To make it complete, its necessary to enforce a wellformedness property over the predicate 
+representation, such that constraints on non-volatile variables can be observed by
+their volatile equivalents.
+
+The implications of this loss of completeness needs to be considered and either accepted
+or a new @{term wp} transformer that preserves the wellformedness property implemented.
+\<close>
+
+definition wf
+  where "wf P \<equiv> \<forall>v p f Fs Vs. (v,p,f) \<in> P \<longrightarrow> 
+              (v,(override_on (override_on p f Fs) v Vs),(override_on f v Vs)) \<in> P"
+
+
+text \<open>Prefix a series of buffers with a constant list\<close>
+definition prefix
+  where "prefix m X p \<equiv> buffers_update (\<lambda>b. \<lambda>y. if y \<in> X then p@(b y) else b y) m"
+
+lemma [simp]:
+  "get (prefix m X [PFO t]) = get m"
+  by (auto simp: prefix_def get_def fun_eq_iff split: option.splits pevent.split)
+
+lemma [simp]:
+  "persistent (prefix m X [PFO t]) = persistent m"
+  by (auto simp: prefix_def fun_eq_iff split: option.splits pevent.split)
+
+lemma [simp]:
+  "get\<^sub>f t (prefix m X [PFO t]) = get\<^sub>f t m"
+  by (auto simp: prefix_def fun_eq_iff get\<^sub>f_def split: option.splits pevent.split)
+
+lemma env_raise:
+  assumes "env (prefix (raise t v p f) X [PFO t]) m"
+  obtains (wrv) x X where "m = prefix (raise t v (p(x := v x)) (f(x := v x))) X [PFO t]" |
+          (wrf) x where "m = prefix (raise t v (p(x := f x)) f) (insert x X) [PFO t]" "v x \<noteq> f x" |
+          (fo) x where "m = prefix (raise t v p f) (X - {x}) [PFO t]"
+  using assms
+proof cases
+  case (pwr x v' l)
+  show ?thesis
+  proof (cases "v x = f x \<or> p x = f x")
+    case True
+    hence "m = prefix (raise t v (p(x := v x)) (f(x := v x))) (if p x \<noteq> f x then insert x X else X) [PFO t]"
+      using pwr by (clarsimp split: if_splits simp: raise_def fun_eq_iff prefix_def)
+    then show ?thesis using wrv by blast
+  next
+    case False
+    hence "m = prefix (raise t v (p(x := f x)) f) (insert x X) [PFO t]"
+      using pwr by (clarsimp split: if_splits simp: prefix_def raise_def fun_eq_iff)
+    then show ?thesis using wrf False by auto
+  qed
+next
+  case (pfo x t' l)
+  hence "m = prefix (raise t v p f) (X - {x}) [PFO t]"
+    by (clarsimp split: if_splits simp: prefix_def raise_def fun_eq_iff)
+  then show ?thesis using fo by auto
+qed
+
+lemma envt_raise:
+  assumes "env\<^sup>*\<^sup>* (prefix (raise t v p f) X [PFO t]) m"
+  obtains Fs Vs X' where "m = prefix (raise t v (override_on (override_on p f Fs) v Vs) (override_on f v Vs)) X' [PFO t]"
+  using assms
+proof (induct)
+  case base
+  show ?case using base[where Fs="{}" and Vs="{}"] by auto
+next
+  case (step m\<^sub>2 m\<^sub>3)
+  show ?case
+  proof (rule step(3), goal_cases)
+    case (1 Fs Vs X')
+    show ?case using step(2) unfolding 1
+    proof (cases rule: env_raise)
+      case (wrv x X)
+      then show ?thesis 
+        using step(4)[where Fs=Fs and Vs="insert x Vs" and X'=X]
+        by (metis override_on_insert) 
+    next
+      case (wrf x)
+      hence e: "x \<notin> Vs" by (auto simp: override_on_def)
+      hence a: "override_on f v Vs x = f x" by (auto simp: override_on_def)
+      have b: "\<And>q f v. (override_on q v Vs)(x := f x) = override_on (q(x:=f x)) v Vs"
+        using e unfolding override_on_def by auto
+      show ?thesis
+        using wrf(1) step(4)[where Fs="insert x Fs" and Vs=Vs and X'="insert x X'"]
+        unfolding override_on_insert a b by blast
+    next
+      case (fo x)
+      then show ?thesis using step(4) by blast
+    qed
+  qed 
+qed
+
+subsection \<open>Implication\<close>
+
+lemma imp_complete:
+  assumes "wf P"
+  assumes "\<forall>m. sat t P m \<longrightarrow> sat t Q m"
+  shows "P \<subseteq> Q"
+proof clarsimp
+  fix v p f
+  assume p: "(v,p,f) \<in> P"
+  let ?m = "prefix (raise t v p f) {} [PFO t]"
+  have "sat t P ?m" using p assms(1) unfolding wf_def sat_def by (clarsimp elim!: envt_raise)
+  hence "sat t Q ?m" using assms by auto
+  thus "(v,p,f) \<in> Q" by (auto simp: sat_def)
+qed
+
+lemma c[simp]:
+  "override_on (p(x := e)) (f(x := e)) V = (override_on p f V)(x := e)"
+  unfolding override_on_def fun_eq_iff by auto
+
+lemma [simp]:
+  "override_on (p(x := f x)) f V = (override_on p f V)(x := f x)"
+  unfolding override_on_def fun_eq_iff by auto
+
+lemma [simp]:
+  "override_on f f Fs = f"
+  by (auto simp: override_on_def)
+
+lemma [simp]:
+  "x \<notin> Vs \<Longrightarrow> override_on f (v(x := e)) Vs = override_on f v Vs"
+  by (auto simp: override_on_def)
+
+lemma d:
+  "x \<in> Vs \<Longrightarrow> override_on (f(x := v x)) (v(x := e))
+      (Vs - {x}) = override_on f v Vs"
+  by (auto simp: override_on_def fun_eq_iff)
+
+lemma [simp]:
+  "(override_on f v (Vs - {x}))(x := e) = (override_on f v Vs)(x := e)"
+  by (auto simp: override_on_def fun_eq_iff)
 
 end
